DAList.thy
@@ -1,0 +1,101 @@
+theory DAList
+  imports "thys/MRBNF_Recursor"
+begin
+
+(* The HOL-Library.DAList entry does not close the context *)
+typedef ('k, 'v) dalist = "{ (xs::('k \<times> 'v) list). distinct (map fst xs) }"
+  by (rule exI[of _ "[]"]) auto
+
+setup_lifting type_definition_dalist
+
+lift_definition map_dalist :: "('k \<Rightarrow> 'k) \<Rightarrow> ('a \<Rightarrow> 'b) \<Rightarrow> ('k, 'a) dalist \<Rightarrow> ('k, 'b) dalist"
+  is "\<lambda>f g x. if inj_on f (fst ` set x) then map (map_prod f g) x else []"
+  by (auto split: if_splits)[1] (simp add: comp_inj_on distinct_map)
+
+lift_definition keys_dalist :: "('k, 'v) dalist \<Rightarrow> 'k set" is "\<lambda>x. fst ` set x" .
+lift_definition vals_dalist :: "('k, 'v) dalist \<Rightarrow> 'v set" is "\<lambda>x. snd ` set x" .
+lift_definition pairs_dalist :: "('k, 'v) dalist \<Rightarrow> ('k \<times> 'v) set" is "set" .
+
+lift_definition dalist_all2 :: "('v \<Rightarrow> 'b \<Rightarrow> bool) \<Rightarrow> ('k, 'v) dalist \<Rightarrow> ('k, 'b) dalist \<Rightarrow> bool"
+  is "\<lambda>R. list_all2 (rel_prod (=) R)" .
+
+mrbnf "('k, 'v) dalist"
+map: map_dalist
+sets:
+  bound: keys_dalist
+  live: vals_dalist
+bd: natLeq
+rel: dalist_all2
+  subgoal
+    apply (rule ext)
+    apply transfer
+    apply auto
+    done
+  subgoal
+    apply (rule ext)
+    apply transfer
+    apply (auto simp: image_image comp_inj_on_iff[symmetric] dest: inj_on_imageI2)
+    done
+  subgoal
+    apply transfer
+    apply (force simp: inj_on_def intro!: list.map_cong)
+    done
+  subgoal
+    apply (rule ext)
+    apply transfer
+    apply (force simp: list.set_map inj_on_def)
+    done
+  subgoal
+    apply (rule ext)
+    apply transfer
+    apply (force simp: list.set_map inj_on_def)
+    done
+      apply (rule infinite_regular_card_order_natLeq)
+  subgoal
+    apply transfer
+    using finite_iff_ordLess_natLeq by blast
+  subgoal
+    apply transfer
+    using finite_iff_ordLess_natLeq by blast
+  subgoal
+    apply (rule predicate2I)
+    apply transfer
+    apply safe
+    apply (subst OO_eq[symmetric, of "(=)"])
+    apply (unfold prod.rel_compp list.rel_compp)
+    apply auto
+    done
+  subgoal for f R
+    apply (transfer fixing: f R)
+    subgoal for xs ys
+      apply (simp only: bij_is_inj[THEN inj_on_subset[OF _ subset_UNIV]] if_True inj_on_id list.in_rel)
+      apply safe
+      subgoal for zs
+        apply (drule arg_cong[where f="map (map_prod (inv f) id)"])
+        apply (force intro!: exI[of _ "map (\<lambda>((a,b),(c,d)). (inv f a,b,d)) zs"] list.map_cong
+          simp: list.map_comp list.map_ident list.set_map prod.map_comp o_def split_beta)
+        done
+      subgoal for zs
+        apply (rule exI[of _ "map (\<lambda>(a,b,c). ((f a,b),(f a,c))) zs"])
+        apply (auto simp: list.map_comp list.set_map prod.map_comp o_def split_beta intro: list.map_cong)
+        done
+      done
+    done
+  done
+
+lift_definition insert_dalist :: "'k \<Rightarrow> 'v \<Rightarrow> ('k, 'v) dalist \<Rightarrow> ('k, 'v) dalist" is
+  "\<lambda>k v x. if k \<in> fst ` set x then x else (k, v) # x"
+  by (auto split: if_splits)
+
+lemma pairs_insert_fresh[simp]: "k \<notin> keys_dalist xs \<Longrightarrow> pairs_dalist (insert_dalist k v xs) = insert (k, v) (pairs_dalist xs)"
+  by transfer auto
+lemma pairs_insert_same[simp]: "k \<in> keys_dalist xs \<Longrightarrow> pairs_dalist (insert_dalist k v xs) = pairs_dalist xs"
+  by transfer auto
+lemma fst_pairs_dalist: "keys_dalist xs = fst ` pairs_dalist xs"
+  by transfer (rule refl)
+
+lift_definition concat_dalist :: "('k, 'v) dalist \<Rightarrow> ('k, 'v) dalist \<Rightarrow> ('k, 'v) dalist"
+  is "\<lambda>xs ys. if fst ` set xs \<inter> fst ` set ys = {} then xs @ ys else []"
+  by auto
+
+end
