thys/POPLmark/POPLmark_1A.thy
@@ -1,0 +1,366 @@
+theory POPLmark_1A
+  imports "../MRBNF_Recursor"
+    "../../DAList" "../Instantiation_Infrastructure/FixedCountableVars"
+    "../Instantiation_Infrastructure/Curry_LFP" 
+    "../Generic_Barendregt_Enhanced_Rule_Induction"
+begin
+
+declare bij_swap[simp]
+
+ML \<open>
+val ctors = [
+  (("TyVar", (NONE : mixfix option)), [@{typ 'var}]),
+  (("Top", (NONE : mixfix option)), []),
+  (("Fun", NONE), [@{typ 'rec}, @{typ 'rec}]),
+  (("Forall", NONE), [@{typ 'bvar}, @{typ 'rec}, @{typ 'brec}])
+]
+
+val spec = {
+  fp_b = @{binding "typ"},
+  vars = [
+    (dest_TFree @{typ 'var}, MRBNF_Def.Free_Var),
+    (dest_TFree @{typ 'bvar}, MRBNF_Def.Bound_Var),
+    (dest_TFree @{typ 'brec}, MRBNF_Def.Live_Var),
+    (dest_TFree @{typ 'rec}, MRBNF_Def.Live_Var)
+  ],
+  binding_rel = [[0]],
+  rec_vars = 2,
+  ctors = ctors,
+  map_b = @{binding vvsubst_typ},
+  tvsubst_b = @{binding tvsubst_typ}
+}
+\<close>
+
+declare [[mrbnf_internals]]
+local_setup \<open>fn lthy =>
+let
+  val lthy' = MRBNF_Sugar.create_binder_datatype spec lthy
+in lthy' end\<close>
+print_theorems
+print_mrbnfs
+
+instance var :: var_typ_pre apply standard 
+  using Field_natLeq infinite_iff_card_of_nat infinite_var
+  by (auto simp add: regularCard_var)
+instance var :: var_dalist apply standard 
+  using Field_natLeq infinite_iff_card_of_nat infinite_var
+  by (auto simp add: regularCard_var)
+
+declare supp_swap_bound[OF cinfinite_imp_infinite[OF typ.UNIV_cinfinite], simp]
+declare typ.rrename_ids[simp] typ.rrename_id0s[simp]
+
+lemma rrename_typ_simps[simp]:
+  fixes f::"'a::var_typ_pre \<Rightarrow> 'a"
+  assumes "bij f" "|supp f| <o |UNIV::'a set|"
+  shows
+    "rrename_typ f (TyVar a) = TyVar (f a)"
+    "rrename_typ f Top = Top"
+    "rrename_typ f (Fun t1 t2) = Fun (rrename_typ f t1) (rrename_typ f t2)"
+    "rrename_typ f (Forall x T1 T2) = Forall (f x) (rrename_typ f T1) (rrename_typ f T2)"
+     apply (unfold TyVar_def Top_def Fun_def Forall_def)
+     apply (rule trans)
+      apply (rule typ.rrename_cctors)
+       apply (rule assms)+
+     defer
+     apply (rule trans)
+      apply (rule typ.rrename_cctors)
+       apply (rule assms)+
+     defer
+     apply (rule trans)
+      apply (rule typ.rrename_cctors)
+       apply (rule assms)+
+     defer
+     apply (rule trans)
+      apply (rule typ.rrename_cctors)
+       apply (rule assms)+
+     defer
+     apply (unfold map_typ_pre_def comp_def Abs_typ_pre_inverse[OF UNIV_I] map_sum.simps
+        map_prod_simp id_def
+      )
+     apply (rule refl)+
+  done
+
+type_synonym type = "var typ"
+type_synonym \<Gamma>\<^sub>\<tau> = "(var, type) dalist"
+
+declare [[inductive_internals]]
+
+notation Fun (infixr "\<rightarrow>" 65)
+notation Forall ("\<forall> _ <: _ . _" [62, 62, 62] 70)
+
+abbreviation in_context :: "var \<Rightarrow> type \<Rightarrow> \<Gamma>\<^sub>\<tau> \<Rightarrow> bool" ("_ <: _ \<in> _" [55,55,55] 60) where
+  "x <: t \<in> \<Gamma> \<equiv> (x, t) \<in> pairs_dalist \<Gamma>"
+abbreviation extend :: "\<Gamma>\<^sub>\<tau> \<Rightarrow> var \<Rightarrow> type \<Rightarrow> \<Gamma>\<^sub>\<tau>" ("_ , _ <: _" [57,57,57] 62) where
+  "\<Gamma>, x<:t \<equiv> insert_dalist x t \<Gamma>"
+abbreviation map_context :: "(var \<Rightarrow> var) \<Rightarrow> \<Gamma>\<^sub>\<tau> \<Rightarrow> \<Gamma>\<^sub>\<tau>" where
+  "map_context f \<equiv> map_dalist f (rrename_typ f)"
+abbreviation dom :: "('k, 'v) dalist \<Rightarrow> 'k set" where "dom \<equiv> keys_dalist"
+abbreviation empty :: "'a set" ("\<emptyset>") where "empty \<equiv> {}"
+abbreviation concat :: "('k, 'v) dalist \<Rightarrow> ('k, 'v) dalist \<Rightarrow> ('k, 'v) dalist" ("_, _" [65,65] 70) where
+  "concat \<equiv> concat_dalist"
+
+inductive Ty :: "\<Gamma>\<^sub>\<tau> \<Rightarrow> type \<Rightarrow> type \<Rightarrow> bool" ("_ \<turnstile> _ <: _" [55,55,55] 60) where
+  SA_Top:         "\<Gamma> \<turnstile> S <: Top"
+| SA_Refl_TVar:   "\<Gamma> \<turnstile> TyVar x <: TyVar x"
+| SA_Trans_TVar:  "\<lbrakk> x<:U \<in> \<Gamma> ; \<Gamma> \<turnstile> U <: T \<rbrakk> \<Longrightarrow> \<Gamma> \<turnstile> TyVar x <: T"
+| SA_Arrow:       "\<lbrakk> \<Gamma> \<turnstile> T\<^sub>1 <: S\<^sub>1 ; \<Gamma> \<turnstile> S\<^sub>2 <: T\<^sub>2 \<rbrakk> \<Longrightarrow> \<Gamma> \<turnstile> S\<^sub>1 \<rightarrow> S\<^sub>2 <: T\<^sub>1 \<rightarrow> T\<^sub>2"
+| SA_All:         "\<lbrakk> \<Gamma> \<turnstile> T\<^sub>1 <: S\<^sub>1 ; \<Gamma>, x<:T\<^sub>1 \<turnstile> S\<^sub>2 <: T\<^sub>2 \<rbrakk> \<Longrightarrow> \<Gamma> \<turnstile> \<forall>x<:S\<^sub>1. S\<^sub>2 <: \<forall>x<:T\<^sub>1 .T\<^sub>2" (* potentially needs "x \<notin> dom \<Gamma>" as assumption *)
+
+thm Ty_def
+declare Ty.intros[intro]
+
+(* instantiating the induction locale *)
+interpretation Small where dummy = "undefined :: var" 
+apply standard
+  apply (simp add: infinite_var)  
+  using var_typ_pre_class.regular by blast
+
+type_synonym T = "\<Gamma>\<^sub>\<tau> \<times> type \<times> type"
+type_synonym V = "var list"
+
+definition Tmap :: "(var \<Rightarrow> var) \<Rightarrow> T \<Rightarrow> T" where
+  "Tmap f \<equiv> map_prod (map_context f) (map_prod (rrename_typ f) (rrename_typ f))"
+fun Tfvars :: "T \<Rightarrow> var set" where
+  "Tfvars (\<Gamma>, T\<^sub>1, T\<^sub>2) = keys_dalist \<Gamma> \<union> \<Union>(FFVars_typ ` vals_dalist \<Gamma>) \<union> FFVars_typ T\<^sub>1 \<union> FFVars_typ T\<^sub>2"
+
+definition Vmap :: "(var \<Rightarrow> var) \<Rightarrow> V \<Rightarrow> V" where 
+  "Vmap \<equiv> map"
+fun Vfvars :: "V \<Rightarrow> var set" where 
+  "Vfvars v = set v"
+
+interpretation Components where dummy = "undefined :: var" and
+Tmap = Tmap and Tfvars = Tfvars
+and Vmap = Vmap and Vfvars = Vfvars 
+apply standard unfolding ssbij_def Tmap_def Vmap_def
+  using small_Un small_def typ.card_of_FFVars_bounds
+         apply (auto simp: typ.FFVars_rrenames dalist.map_id0 map_prod.comp dalist.set_map dalist.map_comp typ.rrename_comp0s inf_A)
+    apply (rule var_typ_pre_class.Un_bound var_typ_pre_class.UN_bound
+        typ.card_of_FFVars_bounds dalist.set_bd[THEN ordLess_ordLeq_trans[OF _ var_typ_pre_class.large]])+
+     apply auto
+    apply (rule sym)
+    apply (rule trans[OF dalist.map_id[symmetric]])
+    apply (rule dalist.map_cong)
+          apply (rule bij_id supp_id_bound refl | assumption)+
+     apply (rule trans[OF id_apply])
+     apply (rule sym)
+     apply (erule ballE)
+      apply assumption
+     apply (erule notE)
+     apply (rule UnI1)+
+     apply assumption
+    apply (rule trans[OF id_apply])
+    apply (rule sym)
+    apply (rule typ.rrename_cong_ids)
+      apply assumption+
+    apply (erule ballE)
+     apply assumption
+    apply (erule notE)
+    apply (rule UnI1, rule UnI1, rule UnI2)
+    apply (rule UN_I)
+     apply assumption+
+   apply (rule typ.rrename_cong_ids)
+      apply assumption+
+    apply (erule ballE)
+     apply assumption
+    apply (erule notE)
+    apply (rule UnI1, rule UnI2)
+     apply assumption
+   apply (rule typ.rrename_cong_ids)
+      apply assumption+
+    apply (erule ballE)
+     apply assumption
+    apply (erule notE)
+    apply (rule UnI2)
+  apply assumption
+  done
+
+definition G :: "(T \<Rightarrow> bool) \<Rightarrow> V \<Rightarrow> T \<Rightarrow> bool" where
+  "G \<equiv> \<lambda>R v t.
+    (v = [] \<and> snd (snd t) = Top)
+  \<or> (\<exists>x. v = [] \<and> fst (snd t) = TyVar x \<and> fst (snd t) = snd (snd t))
+  \<or> (\<exists>x U \<Gamma> T. v = [] \<and> fst t = \<Gamma> \<and> fst (snd t) = TyVar x \<and> snd (snd t) = T \<and> x <: U \<in> \<Gamma> \<and> R (\<Gamma>, U, T))
+  \<or> (\<exists>\<Gamma> T\<^sub>1 S\<^sub>1 S\<^sub>2 T\<^sub>2. v = [] \<and> fst t = \<Gamma> \<and> fst (snd t) = (S\<^sub>1 \<rightarrow> S\<^sub>2) \<and> snd (snd t) = (T\<^sub>1 \<rightarrow> T\<^sub>2) \<and> R (\<Gamma>, T\<^sub>1, S\<^sub>1) \<and> R (\<Gamma>, S\<^sub>2, T\<^sub>2))
+  \<or> (\<exists>\<Gamma> T\<^sub>1 S\<^sub>1 x S\<^sub>2 T\<^sub>2. v = [x] \<and> fst t = \<Gamma> \<and> fst (snd t) = (\<forall>x<:S\<^sub>1. S\<^sub>2) \<and> snd (snd t) = (\<forall>x<:T\<^sub>1. T\<^sub>2) \<and> R (\<Gamma>, T\<^sub>1, S\<^sub>1) \<and> R (\<Gamma>,x<:T\<^sub>1, S\<^sub>2, T\<^sub>2))
+  "
+
+lemma GG_mono: "R \<le> R' \<Longrightarrow> G R v t \<Longrightarrow> G R' v t"
+  unfolding G_def by fastforce
+
+lemma in_context_eqvt:
+  assumes "bij f" "|supp f| <o |UNIV::var set|"
+  shows "x <: T \<in> \<Gamma> \<Longrightarrow> f x <: rrename_typ f T \<in> map_dalist f (rrename_typ f) \<Gamma>"
+  using assms by transfer (auto simp: inj_on_def)
+
+lemma extend_eqvt:
+  assumes "bij f" "|supp f| <o |UNIV::var set|"
+  shows "map_context f (\<Gamma>,x<:T) = map_context f \<Gamma>,f x <: rrename_typ f T"
+  using assms by transfer (auto simp: inj_on_def image_iff)
+
+lemma GG_equiv: "ssbij \<sigma> \<Longrightarrow> G R v t \<Longrightarrow> G (\<lambda>t'. R (Tmap (inv \<sigma>) t')) (Vmap \<sigma> v) (Tmap \<sigma> t)"
+  unfolding G_def
+  apply (elim disjE)
+  subgoal
+    apply (rule disjI1)
+    apply (cases t)
+    unfolding ssbij_def Tmap_def Vmap_def by simp
+  subgoal
+    apply (rule disjI2, rule disjI1)
+    apply (erule exE)
+    apply (elim conjE)
+    subgoal for x
+      apply (cases t)
+      unfolding ssbij_def Tmap_def Vmap_def by auto
+    done
+  subgoal
+    apply (rule disjI2, rule disjI2, rule disjI1)
+    apply (elim exE conjE)
+    subgoal for x U \<Gamma> T
+      apply (rule exI)
+      apply (rule exI[of _ "rrename_typ \<sigma> U"])
+      apply (rule exI[of _ "map_dalist \<sigma> (rrename_typ \<sigma>) \<Gamma>"])
+      apply (rule exI[of _ "rrename_typ \<sigma> T"])
+      apply (cases t)
+      unfolding ssbij_def Tmap_def Vmap_def
+      by (auto simp: in_context_eqvt dalist.map_comp supp_inv_bound
+          typ.rrename_comps typ.rrename_comp0s dalist.map_id)
+    done
+  subgoal
+    apply (rule disjI2, rule disjI2, rule disjI2, rule disjI1)
+    apply (elim exE conjE)
+    subgoal for \<Gamma> T1 S1 S2 T2
+      apply (rule exI[of _ "map_dalist \<sigma> (rrename_typ \<sigma>) \<Gamma>"])
+      apply (rule exI[of _ "rrename_typ \<sigma> T1"])
+      apply (rule exI[of _ "rrename_typ \<sigma> S1"])
+      apply (rule exI[of _ "rrename_typ \<sigma> S2"])
+      apply (rule exI[of _ "rrename_typ \<sigma> T2"])
+      apply (cases t) unfolding ssbij_def Tmap_def Vmap_def
+      by (auto simp: in_context_eqvt dalist.map_comp supp_inv_bound
+          typ.rrename_comps typ.rrename_comp0s dalist.map_id)
+    done
+  apply (rule disjI2)+
+  apply (elim exE conjE)
+  subgoal for \<Gamma> T1 S1 x S2 T2
+          apply (rule exI[of _ "map_dalist \<sigma> (rrename_typ \<sigma>) \<Gamma>"])
+      apply (rule exI[of _ "rrename_typ \<sigma> T1"])
+    apply (rule exI[of _ "rrename_typ \<sigma> S1"])
+    apply (rule exI)
+      apply (rule exI[of _ "rrename_typ \<sigma> S2"])
+    apply (rule exI[of _ "rrename_typ \<sigma> T2"])
+    apply (cases t) unfolding ssbij_def Tmap_def Vmap_def
+    apply (auto simp: in_context_eqvt dalist.map_comp supp_inv_bound typ.FFVars_rrenames
+          typ.rrename_comps typ.rrename_comp0s dalist.map_id extend_eqvt dalist.set_map
+      )
+    done
+  done
+
+lemma fresh: "\<exists>xx. xx \<notin> Tfvars t"  
+  by (metis emp_bound equals0D imageI inf.commute inf_absorb2 small_Tfvars small_def small_ssbij subsetI)
+
+lemma Forall_rrename: 
+  assumes "bij \<sigma>" "|supp \<sigma>| <o |UNIV::'a set|" shows "
+ (\<And>a'. a'\<in>FFVars_typ T2 - {x::'a::var_typ_pre} \<Longrightarrow> \<sigma> a' = a') \<Longrightarrow> Forall x T1 T2 = Forall (\<sigma> x) T1 (rrename_typ \<sigma> T2)"
+  apply (unfold Forall_def)
+  apply (unfold typ.TT_injects0)
+  apply (unfold set3_typ_pre_def set2_typ_pre_def comp_def Abs_typ_pre_inverse[OF UNIV_I] map_sum.simps
+    map_prod_simp sum_set_simps prod_set_simps cSup_singleton Un_empty_left Un_empty_right
+    Union_empty image_insert image_empty map_typ_pre_def id_def
+  )
+  apply (rule exI[of _ \<sigma>])
+  apply (rule conjI assms)+
+   apply (unfold id_on_def atomize_all atomize_imp)[1]
+   apply (rule impI)
+   apply assumption
+  apply (rule refl)
+  done
+
+lemma swap_idemp[simp]: "id(x := x) = id" by auto
+lemma swap_left: "(id(x := xx, xx := x)) x = xx" by simp
+
+lemma GG_fresh:
+  "(\<forall>\<sigma> t. ssbij \<sigma> \<and> R t \<longrightarrow> R (Tmap \<sigma> t)) \<Longrightarrow> G R v t \<Longrightarrow>
+  \<exists>w. Vfvars w \<inter> Tfvars t = {} \<and> G R w t"
+  using fresh[of t] unfolding G_def Tmap_def Vmap_def apply safe
+  subgoal by (rule exI[of _ "[]"]) auto
+  subgoal by (rule exI[of _ "[]"]) auto
+  subgoal by (rule exI[of _ "[]"]) auto
+  subgoal by (rule exI[of _ "[]"]) fastforce
+  subgoal for xx \<Gamma> T\<^sub>1 S\<^sub>1 x S\<^sub>2 T\<^sub>2
+    apply (rule exI[of _ "[xx]"])
+    apply (rule conjI)
+    subgoal by auto
+    apply (rule disjI2)+
+    apply (rule exI[of _ "fst t"])
+  apply (rule exI[of _ "T\<^sub>1"])
+    apply (rule exI[of _ "S\<^sub>1"])
+    apply (rule exI[of _ "xx"])
+    apply (rule exI[of _ "rrename_typ (id(x:=xx,xx:=x)) S\<^sub>2"])
+    apply (rule exI[of _ "rrename_typ (id(x:=xx,xx:=x)) T\<^sub>2"])
+    apply (cases t) apply simp
+    apply (intro conjI)
+    subgoal apply (subst Forall_rrename[of "id(x:=xx,xx:=x)"]) by auto
+    subgoal
+      apply (elim conjE)
+        apply (subst Forall_rrename[of "id(x:=xx,xx:=x)"])
+      by auto
+    sorry
+  done
+
+interpretation Induct where dummy = "undefined :: var"
+  and Tmap = Tmap and Tfvars = Tfvars and Vmap = Vmap and Vfvars = Vfvars and G = G
+  apply standard
+  using GG_mono GG_equiv GG_fresh by auto
+print_theorems
+
+lemma Ty_I: "Ty \<Gamma> T1 T2 = I (\<Gamma>, T1, T2)"
+  unfolding Ty_def I_def lfp_curry3 apply(rule arg_cong2[of _ _ _ _ lfp], simp_all)
+  unfolding fun_eq_iff G_def apply safe
+           apply auto
+  by blast
+
+corollary Ty_strong_induct[consumes 1, case_names Bound SA_Top SA_Refl_TVar SA_Trans_TVar SA_Arrow SA_All]:
+  "\<Gamma> \<turnstile> S <: T \<Longrightarrow>
+  \<forall>\<rho>. |K \<rho>| <o |UNIV::var set| \<Longrightarrow>  
+  (\<And>\<Gamma> S \<rho>. P \<Gamma> S Top \<rho>) \<Longrightarrow>
+  (\<And>\<Gamma> x \<rho>. P \<Gamma> (TyVar x) (TyVar x) \<rho>) \<Longrightarrow>
+  (\<And>x U \<Gamma> T \<rho>. x <: U \<in> \<Gamma> \<Longrightarrow> \<Gamma> \<turnstile> U <: T \<Longrightarrow> \<forall>\<rho>. P \<Gamma> U T \<rho> \<Longrightarrow> P \<Gamma> (TyVar x) T \<rho>) \<Longrightarrow>
+  (\<And>\<Gamma> T\<^sub>1 S\<^sub>1 S\<^sub>2 T\<^sub>2 \<rho>. \<Gamma> \<turnstile> T\<^sub>1 <: S\<^sub>1 \<Longrightarrow> \<forall>\<rho>. P \<Gamma> T\<^sub>1 S\<^sub>1 \<rho> \<Longrightarrow> \<Gamma> \<turnstile> S\<^sub>2 <: T\<^sub>2 \<Longrightarrow> \<forall>\<rho>. P \<Gamma> S\<^sub>2 T\<^sub>2 \<rho> \<Longrightarrow> P \<Gamma> (S\<^sub>1 \<rightarrow> S\<^sub>2) (T\<^sub>1 \<rightarrow> T\<^sub>2) \<rho>) \<Longrightarrow>
+  (\<And>\<Gamma> T\<^sub>1 S\<^sub>1 x S\<^sub>2 T\<^sub>2 \<rho>. x \<notin> K \<rho> \<Longrightarrow> \<Gamma> \<turnstile> T\<^sub>1 <: S\<^sub>1 \<Longrightarrow> \<forall>\<rho>. P \<Gamma> T\<^sub>1 S\<^sub>1 \<rho> \<Longrightarrow> \<Gamma> , x <: T\<^sub>1 \<turnstile> S\<^sub>2 <: T\<^sub>2 \<Longrightarrow> \<forall>\<rho>. P (\<Gamma> , x <: T\<^sub>1) S\<^sub>2 T\<^sub>2 \<rho> \<Longrightarrow> P \<Gamma> (\<forall> x <: S\<^sub>1 . S\<^sub>2) (\<forall> x <: T\<^sub>1 . T\<^sub>2) \<rho>) \<Longrightarrow>
+ \<forall>\<rho>. P \<Gamma> S T \<rho>"
+  unfolding Ty_I
+  apply (rule allI)
+  subgoal for \<rho>
+    apply (subgoal_tac "case (\<Gamma>, S, T) of (\<Gamma>, S, T) \<Rightarrow> P \<Gamma> S T \<rho>")
+    subgoal by auto
+    subgoal apply (rule BE_induct[where R="\<lambda>p (\<Gamma>,S,T). P \<Gamma> S T p" and Pfvars = K])
+        apply (unfold small_def)[1]
+        apply (erule allE)
+        apply assumption+
+      unfolding G_def by (auto split: if_splits)
+    done
+  done
+
+(********************* Actual formalization ************************)
+lemma Ty_refl: "\<Gamma> \<turnstile> T <: T"
+  by (induction arbitrary: \<Gamma>) auto
+
+lemma Ty_permute: "\<lbrakk> \<Gamma> \<turnstile> S <: T ; pairs_dalist \<Gamma> = pairs_dalist \<Delta> \<rbrakk> \<Longrightarrow> \<Delta> \<turnstile> S <: T"
+proof (induction \<Gamma> S T arbitrary: \<Delta> rule: Ty.induct)
+  case (SA_All \<Gamma> T\<^sub>1 S\<^sub>1 x S\<^sub>2 T\<^sub>2)
+  then have "keys_dalist \<Gamma> = keys_dalist \<Delta>" by (metis fst_pairs_dalist)
+  then have "pairs_dalist (\<Gamma>, x <: T\<^sub>1) = pairs_dalist (\<Delta>, x <: T\<^sub>1)"
+    by (metis SA_All.prems pairs_insert_fresh pairs_insert_same)
+  then show ?case using SA_All by blast
+qed auto
+
+lemma in_concat_dalist[simp]: "keys_dalist xs \<inter> keys_dalist ys = {} \<Longrightarrow> pairs_dalist (concat_dalist xs ys) = pairs_dalist xs \<union> pairs_dalist ys"
+  by transfer auto
+
+lemma Ty_weakening: "\<lbrakk> \<Gamma> \<turnstile> S <: T ; dom \<Gamma> \<inter> dom \<Delta> = \<emptyset> \<rbrakk> \<Longrightarrow> \<Gamma>,\<Delta> \<turnstile> S <: T"
+proof (binder_induction \<Gamma> S T avoiding: \<Delta> rule: Ty_strong_induct)
+(*proof (induction \<Gamma> S T arbitrary: \<Delta> rule: Ty.induct)
+  case (SA_All \<Gamma> T\<^sub>1 S\<^sub>1 x S\<^sub>2 T\<^sub>2)
+  then show ?case sorry
+qed auto*)
+  oops
+
+end
